

## Problem 1

Show that Equation 8 in Lecture 3, i.e, the partial derivative of  $J(\beta)$  with respect to  $\beta_j$  is,

$$\frac{\partial}{\partial \beta_j} = \frac{1}{N} \sum_{i=1}^N (\sigma(\beta^T \mathbf{x}_i) - y_i) x_{ij}$$

### *My Solution:*

First note that  $J(\hat{\beta}) = -\frac{1}{N} \sum_{i=1}^N [y_i \log(p_i) + (1 - y_i) \log(1 - p_i)]$ . Then we also know that  $p_i = \sigma(\beta^T \mathbf{x}_i)$  thus if we let  $t_i = \beta^T \mathbf{x}_i$  then  $p_i = \sigma(t_i) = \frac{1}{1+e^{-t_i}}$ . Briefly note that  $t_i = \beta_0 + \beta_1 x_{i1} + \dots + \beta_N x_{iN}$  and thus  $t_i$  is a function of  $\beta_j$ . Here are two facts I will use to show my solution,

$$\frac{d}{dt_i} \sigma(t_i) = \frac{d}{dt_i} \left[ \frac{1}{1 + e^{-t_i}} \right] = \sigma(t_i)(1 - \sigma(t_i)) \quad (1)$$

$$\frac{\partial t_i}{\partial \beta_j} = x_{ij} \quad (2)$$

Now I will replace every  $p_i$  with  $\sigma(t_i)$  as they are equivalent expressions,

$$J(\beta) = -\frac{1}{N} \sum_{i=1}^N [y_i \log(\sigma(t_i)) + (1 - y_i) \log(1 - \sigma(t_i))]$$

Note then,

$$\frac{\partial}{\partial \beta_j} \left[ -\frac{1}{N} \sum_{i=1}^N y_i \log(\sigma(t_i)) + (1 - y_i) \log(1 - \sigma(t_i)) \right] \quad (3)$$

$$\left[ -\frac{1}{N} \sum_{i=1}^N y_i \frac{\partial}{\partial \beta_j} \log(\sigma(t_i)) + (1 - y_i) \frac{\partial}{\partial \beta_j} \log(1 - \sigma(t_i)) \right] \quad (4)$$

Examining each partial independently I will use the fact that  $\frac{d}{dx} \log(f(x)) = \frac{f'(x)}{f(x)}$ ,

$$\frac{\partial}{\partial \beta_j} \log(\sigma(t_i)) = \frac{1}{\sigma(t_i)} \cdot \frac{\partial}{\partial \beta_j} \sigma(t_i)$$

and,

$$\frac{\partial}{\partial \beta_j} \log(1 - \sigma(t_i)) = \frac{1}{1 - \sigma(t_i)} \cdot \frac{\partial}{\partial \beta_j} 1 - \sigma(t_i) = -\frac{1}{1 - \sigma(t_i)} \cdot \frac{\partial}{\partial \beta_j} \sigma(t_i)$$

Now we can rewrite (3) such that each term will have  $\frac{\partial}{\partial \beta_j} \sigma(t_i)$  in common,

$$-\frac{1}{N} \sum_{i=1}^N \left[ \frac{y_i}{\sigma(t_i)} - \frac{1-y_i}{1-\sigma(t_i)} \right] \cdot \frac{\partial}{\partial \beta_j} \sigma(t_i)$$

But note that we will apply the chain rule for  $\frac{\partial}{\partial \beta_j} \sigma(t_i)$  given  $t_i = \beta^T \mathbf{x}_i = \sum_{j=1}^N \beta_j x_{ij}$  thus  $\frac{\partial t_i}{\partial \beta_j} = x_{ij}$ . Further, using the fact that  $\frac{d}{dt} \sigma(t) = \frac{d}{dt} \left[ \frac{1}{1+e^{-t}} \right] = \sigma(t)(1-\sigma(t))$ ,

$$-\frac{1}{N} \sum_{i=1}^N \left[ \frac{y_i}{\sigma(t_i)} - \frac{1-y_i}{1-\sigma(t_i)} \right] \cdot (\sigma(t_i)(1-\sigma(t_i))) \cdot x_{ij}$$

$$-\frac{1}{N} \sum_{i=1}^N \left[ \frac{y_i \cdot \sigma(t_i)(1-\sigma(t_i))}{\sigma(t_i)} - \frac{(1-y_i) \cdot \sigma(t_i)(1-\sigma(t_i))}{1-\sigma(t_i)} \right] \cdot x_{ij}$$

Note the above in red will cancel

$$-\frac{1}{N} \sum_{i=1}^N [y_i - y_i \sigma(t_i) - \sigma(t_i) + y_i \sigma(t_i)] \cdot x_{ij}$$

Therefore,

$$\frac{\partial}{\partial \beta_j} J(\beta) = \frac{1}{N} \sum_{i=1}^N (\sigma(t_i) - y_i) x_{ij}$$

But note  $t_i = \beta^T \mathbf{x}_i$  thus,

$$\frac{\partial}{\partial \beta_j} J(\beta) = \frac{1}{N} \sum_{i=1}^N (\sigma(\beta^T \mathbf{x}_i) - y_i) x_{ij}$$

as desired.

## Problem 2

Consider the softmax regression. The number of data instances  $N$ , and the number of classes is  $K$

**Part a. What is the value of  $\sum_{k=1}^K y_k^{(i)}$  is defined in lecture 4.**

Consider the following objective function,  $J(B) = -\frac{1}{N} \sum_{i=1}^N \sum_{k=1}^K y_k^{(i)} \log(p_k^{(i)})$ .  $y_k^{(i)}$  is the target probability that the  $i$ th instance belongs to class  $k$ . For the correct class  $y_k^{(i)}$  is 1 and zero for all other classes implying that the sum is 1.

Therefore,  $\sum_{k=1}^K y_k^{(i)} = 1$ .

---

**Part b.** Let  $t_k = s_k(x_i)$  so  $p_k$  can be rewritten as:

$$p_k^{(i)} = \frac{\exp(t_k)}{\sum_{j=1}^K \exp(t_j)}$$

Let  $\bar{k}$ ,  $1 \leq \bar{k} \leq K$ , be another index. Show that,

$$\frac{1}{p_k^{(i)}} \frac{\partial p_k^{(i)}}{\partial t_{\bar{k}}} = \begin{cases} -p_{\bar{k}}^{(i)}, & \text{if } k \neq \bar{k} \\ 1 - p_{\bar{k}}^{(i)} = 1 - p_{\bar{k}}^{(i)}, & \text{if } k = \bar{k} \end{cases}$$

---

**My Solution:**

**Case 1: Let  $k = \bar{k}$**

Then note that for  $f(x) = \frac{g(x)}{h(x)} \Rightarrow f'(x) = \frac{g'(x)h(x) - h'(x)g(x)}{[h(x)]^2}$

$$p_k^{(i)} = \frac{e^{t_k}}{\sum_{j=1}^K e^{t_j}}$$

So let  $g(x) = e^{t_k}$  and  $h(x) = \sum_{j=1}^K e^{t_j}$ ,

$$g'(x) = \frac{\partial}{\partial t_k} e^{t_k} = e^{t_k}$$

$$h'(x) = \frac{\partial}{\partial t_k} \sum_{j=1}^K e^{t_j} = \frac{\partial}{\partial t_k} (e^{t_1} + e^{t_2} + \dots + e^{t_{k-1}} + \color{red}{e^{t_k}} + e^{t_{k+1}} + \dots + e^{t_K}) = e^{t_k}$$

$$\frac{\partial}{\partial t_k} p_k^{(i)} = \frac{e^{t_k} \sum_{j=1}^K e^{t_j} - e^{t_k} e^{t_k}}{[\sum_{j=1}^K e^{t_j}]^2}$$

$$\frac{\partial}{\partial t_k} p_k^{(i)} = \frac{e^{t_k} \sum_{j=1}^K e^{t_j}}{[\sum_{j=1}^K e^{t_j}]^2} - \frac{(e^{t_k})^2}{[\sum_{j=1}^K e^{t_j}]^2}$$

Note the definition of  $p_k^{(i)} = \frac{e^{t_k}}{\sum_{j=1}^K e^{t_j}}$

Therefore, when  $k = \bar{k}$  then  $\frac{\partial p_{\bar{k}}^{(i)}}{\partial t_{\bar{k}}} = p_{\bar{k}}^{(i)} - (p_{\bar{k}}^{(i)})^2 = p_{\bar{k}}^{(i)}(1 - p_{\bar{k}}^{(i)})$

**Case 2: Let  $k \neq \bar{k}$**

$$p_k^{(i)} = \frac{e^{t_k}}{\sum_{j=1}^K e^{t_j}}$$

Let  $g(x) = e^{t_k}$  and  $h(x) = \sum_{j=1}^K e^{t_j}$

$$\begin{aligned}
g'(x) &= \frac{\partial}{\partial t_{\bar{k}}} e^{t_k} = 0 \\
h'(x) &= \frac{\partial}{\partial t_{\bar{k}}} (e^{t_1} + \dots + e^{\bar{k}-1} + e^{\bar{k}} + e^{\bar{k}+1} + \dots + e^{t_K}) = e^{t_{\bar{k}}} \\
\frac{\partial}{\partial t_{\bar{k}}} p_k^{(i)} &= \frac{0(\sum_{j=1}^K e^{t_j}) - e^{t_{\bar{k}}} e^{t_k}}{[\sum_{j=1}^K e^{t_j}]^2} = -\frac{e^{t_{\bar{k}}}}{\sum_{j=1}^K e^{t_j}} \frac{e^{t_k}}{\sum_{j=1}^K e^{t_j}} = -p_{\bar{k}}^{(i)} p_k^{(i)}
\end{aligned}$$

Therefore, when  $k \neq \bar{k}$  then  $\frac{\partial}{\partial t_{\bar{k}}} p_k^{(i)} = -p_{\bar{k}}^{(i)} p_k^{(i)}$ .  
Giving,

$$\frac{\partial p_k^{(i)}}{\partial t_{\bar{k}}} = \begin{cases} -p_{\bar{k}}^{(i)} p_k^{(i)}, & \text{if } k \neq \bar{k} \\ p_k^{(i)} (1 - p_k^{(i)}) = p_k^{(i)} (1 - p_{\bar{k}}^{(i)}), & \text{if } k = \bar{k} \end{cases}$$

If we bring out the reciprocal of  $p_k^{(i)}$  for simplification we get,

$$\frac{1}{p_k^{(i)}} \frac{\partial p_k^{(i)}}{\partial t_{\bar{k}}} = \begin{cases} -p_{\bar{k}}^{(i)}, & \text{if } k \neq \bar{k} \\ 1 - p_{\bar{k}}^{(i)} = 1 - p_k^{(i)}, & \text{if } k = \bar{k} \end{cases}$$

as desired.

---

**part c.** Show  $J(B) = -\frac{1}{N} \sum_{i=1}^N \sum_{k=1}^K y_k^{(i)} \log(p_k^{(i)})$  holds,

$$\nabla_{\beta^{\bar{k}}} J(B) = \frac{1}{N} \sum_{i=1}^N (p_{\bar{k}}^{(i)} - y_{\bar{k}}^{(i)}) \mathbf{x}_i$$


---

**My Solution:**

Set-Up: Note that  $J(B)$  is a function of  $p_{\bar{k}}^{(i)}$  and  $p_{\bar{k}}^{(i)}$  is a function of  $t_{\bar{k}}$  in which  $t_{\bar{k}} = x_i^T \beta^{\bar{k}}$  and is a function of  $\beta^{\bar{k}}$ . Therefore, we will use the chain rule and for reference, we will address each layer of  $J(B)$  as follows,

$$\frac{\partial J(B)}{\partial p_k^{(i)}} \frac{\partial p_k^{(i)}}{\partial t_{\bar{k}}} \frac{\partial t_{\bar{k}}}{\partial \beta^{\bar{k}}}$$

Part a. gives that the  $\sum_{k=1}^K y_k^{(i)} = 1$ .

Part b. gives that

$$\frac{1}{p_k^{(i)}} \frac{\partial p_k^{(i)}}{\partial t_{\bar{k}}} = \begin{cases} -p_{\bar{k}}^{(i)}, & \text{if } k \neq \bar{k} \\ 1 - p_{\bar{k}}^{(i)} = 1 - p_k^{(i)}, & \text{if } k = \bar{k} \end{cases}$$

First note that  $\frac{d}{dx} \log(x) = \frac{1}{x}$ ,

$$\frac{\partial J(B)}{\partial p_k^{(i)}} = -\frac{1}{N} \sum_{i=1}^N \sum_{k=1}^K \frac{y_k^{(i)}}{p_k^{(i)}}$$

Second note we have arrived at the fact established in b  $\frac{1}{p_k^{(i)}} \frac{\partial p_k^{(i)}}{\partial t_{\bar{k}}}$ ,

$$\frac{\partial J(B)}{\partial p_k^{(i)}} \frac{\partial p_k^{(i)}}{\partial t_{\bar{k}}} = -\frac{1}{N} \sum_{i=1}^N \sum_{k=1}^K \frac{y_k^{(i)}}{p_k^{(i)}} \frac{\partial p_k^{(i)}}{\partial t_{\bar{k}}}$$

Third, note we are considering  $k = \bar{k}$  that is  $y_{\bar{k}}^{(i)}$  is our target probability and for the correct class,  $\bar{k}$ , this is 1 and for all other classes the value is zero.

$$\frac{\partial J(B)}{\partial p_k^{(i)}} \frac{\partial p_k^{(i)}}{\partial t_{\bar{k}}} = -\frac{1}{N} \sum_{i=1}^N (\sum_{k \neq \bar{k}} y_k^{(i)} (-p_k^{(i)}) + y_{\bar{k}}^{(i)} (1 - p_{\bar{k}}^{(i)}))$$

Note above that  $y_k^{(i)} (-p_k^{(i)})$  will be zero since this is a one hot encoded vector.

Also note for  $k = \bar{k}$  we are just have  $y_{\bar{k}}^{(i)}$ .

Leaving us with the following expression (after distributing the negative sign),

$$\frac{\partial J(B)}{\partial p_k^{(i)}} \frac{\partial p_k^{(i)}}{\partial t_{\bar{k}}} = \frac{1}{N} \sum_{i=1}^N (p_{\bar{k}}^{(i)} - y_{\bar{k}}^{(i)})$$

Fourth, note that  $t_{\bar{k}} = s_{\bar{k}}(\hat{x}_i) = \hat{x}_i^T \beta^{(\bar{k})}$  thus  $\frac{\partial t_{\bar{k}}}{\partial \beta^{(\bar{k})}} = \mathbf{x}_i$

$$\frac{\partial J(B)}{\partial p_k^{(i)}} \frac{\partial p_k^{(i)}}{\partial t_{\bar{k}}} \frac{\partial t_{\bar{k}}}{\partial \beta^{(\bar{k})}} = \nabla_{\beta^{(\bar{k})}} J(B) = \frac{1}{N} \sum_{i=1}^N (p_{\bar{k}}^{(i)} - y_{\bar{k}}^{(i)}) \mathbf{x}_i$$

as desired.

---